progress toward better semantics

theories/continuations.v
@@ -2,6 +2,11 @@ Require Import syntax.
 Require Import Sorting.Permutation.
 Import List.ListNotations.
 Open Scope list_scope.
+Require Import sequences.
+Require Import Lia.
+
+
+(* Definition of continuaton semantics for the catala programming language. *)
 
 Inductive result :=
   | RValue (v: value)
@@ -10,7 +15,7 @@ Inductive result :=
 .
 
 Inductive cont :=
-  | CAppL (t1: term) (* [t1 \square] *)
+  (* | CAppL (t1: term) (* [t1 \square] *) *) (* cannot happend*)
   | CAppR (t2: term) (* [\square t2] *)
   | CClosure (t_cl: {bind term}) (sigma_cl: var -> value)
     (* [Clo(x, t_cl, sigma_cl) \sigma] Since we are using De Bruijn indices, there is no variable x. *)
@@ -150,11 +155,48 @@ Inductive cred: state -> state -> Prop :=
     cred
       (mode_eval Empty kappa sigma)
       (mode_cont kappa sigma REmpty)
+  
+  | cred_value_intr:
+    forall v kappa sigma,
+    cred
+      (mode_eval (Value v) kappa sigma)
+      (mode_cont kappa sigma (RValue v))
 .
 
-Tactic Notation "admit" := admit.
-Tactic Notation "admit" string(x):= admit.
 
+
+Tactic Notation "admit" := admit.
+Tactic Notation "admit" string(x) := admit.
+
+Section CRED_PROPERTIES.
+
+Definition stack s :=
+  match s with
+  | mode_eval _ k _ => k
+  | mode_cont k _ _ => k
+  end.
+
+Theorem cred_progress s:
+  (exists s', cred s s') \/ stack s = [].
+Proof.
+  induction s.
+  * induction e; try solve [left; eexists; econstructor].
+    - admit "todo: add an interpretation for free variables".
+    - admit "todo: add an interpretation of binary operators".
+  * match goal with [v: list cont |- _] => induction v; try solve [left; eexists; econstructor|simpl; eauto] | _ => idtac end;
+    match goal with [v: cont |- _] => induction v; try solve [left; eexists; econstructor|simpl; eauto] | _ => idtac end;
+    match goal with [v: result |- _] => induction v; try solve [left; eexists; econstructor|simpl; eauto] | _ => idtac end;
+    match goal with [v: value |- _] => induction v; try solve [left; eexists; econstructor|simpl; eauto] | _ => idtac end;
+    match goal with [v: option value |- _] => induction v; try solve [left; eexists; econstructor|simpl; eauto] | _ => idtac end;
+    match goal with [v: list term |- _] => induction v; try solve [left; eexists; econstructor|simpl; eauto] | _ => idtac end;
+    match goal with [v: bool |- _] => induction v; try solve [left; eexists; econstructor|simpl; eauto] | _ => idtac end.
+    all: try solve[left; eexists; econstructor; repeat intro; discriminate].
+    - admit "typing error on the function application.".
+    - admit "typing error on the function application.".
+    - admit "typing error on the function application.".
+    - admit "typing error on the justification".
+    - admit "typing error on the justification".
+Admitted.
 
 Theorem cred_deterministic (s s1' s2': state):
   cred s s1' -> cred s s2' -> s1' = s2'.
@@ -169,19 +211,6 @@ Proof.
   * specialize H with None [] tj tc. destruct H. eauto.
 Qed.
 
-Definition stack_empty s :=
-  match s with
-  | mode_eval _ [] _ =>
-    true
-  | mode_cont [] _ _ =>
-    true
-  | _ => false
-  end.
-
-Require Import sequences.
-
-Check irred.
-
 Theorem cred_stack_empty_irred:
   forall sigma v,
     irred cred (mode_cont [] sigma v)
@@ -191,17 +220,31 @@ Proof.
   inversion H.
 Qed.
 
-Theorem cred_star_deterministc s sigma v :
+
+
+Theorem cred_star_deterministic s1 s2 s2':
+  star cred s1 s2 ->
+  star cred s1 s2' ->
+  irred cred s2 ->
+  irred cred s2' ->
+  s2 = s2'.
+Proof.
+  intros; eapply finseq_unique; eauto using cred_deterministic.
+Qed.
+
+
+Theorem cred_star_deterministic_contempty s sigma v :
   star cred s (mode_cont [] sigma v) ->
   forall sigma' v', star cred s (mode_cont [] sigma' v') ->
   sigma = sigma' /\ v = v'.
 Proof.
   intros.
   assert (mode_cont [] sigma v = (mode_cont [] sigma' v')).
-  { eapply finseq_unique; eauto using cred_deterministic, cred_stack_empty_irred.
-  }
-  match goal with [h: mode_cont _ _ _ = mode_cont _ _ _ |- _] => injection h end; eauto.
+  { eapply cred_star_deterministic; eauto using cred_stack_empty_irred. }
+  match goal with [h: mode_cont _ _ _ = mode_cont _ _ _ |- _] =>
+  injection h end; eauto.
 Qed.
+
 
 Definition append_stack s kappa2 :=
   match s with
@@ -212,11 +255,11 @@ Definition append_stack s kappa2 :=
   end
 .
 
+(* Properties of append_stack *)
 
-(* Main Lemma about stack extending *)
 Theorem append_stack_stable s s':
-  cred s s'
-  ->
+  (* If you can do a transition, then you can do the same transition with additional informations on the stack. *)
+  cred s s' ->
   forall k,
   cred (append_stack s k) (append_stack s' k).
 Proof.
@@ -229,13 +272,124 @@ Theorem append_stack_stable_star s s':
   forall k,
   star cred (append_stack s k) (append_stack s' k).
 Proof.
-  induction 1.
+  induction 1; intros.
   * eauto with sequences.
-  * intros.
-    eapply star_step.
-    { eapply append_stack_stable; eauto. }
-    { eapply IHstar. }
+  * eapply star_step; eauto using append_stack_stable.
 Qed.
+
+Lemma append_stack_inv:
+  forall s1 s2 kappa2,
+  s1 = append_stack s2 (kappa2) ->
+  exists kappa1, stack s1 = kappa1 ++ kappa2.
+Proof.
+  induction s1; induction s2; simpl; intros.
+  all: try solve [injection H; intros; subst; eexists; eauto ].
+  all: try solve [discriminate].
+Qed.
+
+(* conversly, if we have a transition *)
+Theorem bottom_stack_unmodified_cred s1 s2 kappa:
+  cred (append_stack s1 kappa) s2 ->
+  List.length (stack (append_stack s1 kappa)) >= List.length kappa ->
+  exists s2', s2 = append_stack s2' kappa.
+Proof.
+  remember (append_stack s1 kappa) as s1'.
+  induction 1; subst; simpl; intros Hlen; match goal with [h: (_ = append_stack _ _) |- _] => pose proof append_stack_inv _ _ _ h as [kappa']; simpl in *; subst end.
+  all: try match goal with [ |- context [_ ++ _]] => admit end.
+Qed.
+
+Theorem bottom_stack_unmodified s1 s2 kappa p:
+  star
+    (fun a b => cred a b /\ p a)
+    s1 s2
+  -> 
+  exists s1', s1 = append_stack s1' kappa ->
+  exists s2', s1 = append_stack s2' kappa.
+Proof.
+  induction 1 as [|a b c [Hred Hp] Hstar IHstar].
+  * eauto.
+  * induction H.
+
+
+Open Scope nat.
+
+Require Import Lia.
+
+From Catala Require Import tactics.
+
+Lemma technical_lemma:
+  forall s1 s2,
+  cred s1 s2 ->
+  Nat.ltb (stack_length s2) (stack_length s1) = true ->
+  exists kappa sigma v,
+  s1 = mode_cont kappa sigma v
+  .
+Proof.
+  induction 1; simpl; eauto.
+  all: admit alain "All cases are trivially true by computation".
+Admitted.
+
+Open Scope nat_scope.
+
+Lemma general_inversion_lemma:
+  forall x k sigma v',
+  star cred
+    (mode_eval x [k] sigma)
+    (mode_cont [] sigma v')
+  ->
+  exists v,
+  star cred 
+    (mode_eval x [k] sigma)
+    (mode_cont [] sigma v).
+Proof.
+  intros.
+  destruct (takewhile (fun s => Nat.ltb 0  (stack_length s) ) H).
+  - eauto.
+  - destruct H0.
+    simpl in H1.
+    exfalso; discriminate.
+  - destruct H0 as [s [Hs1 [Hs2 Hs3]]].
+    induction Hs1 using star_ind_n1.
+    * eauto.
+    *  
+      (* I know cred y z and stack_length y > stack_length z and stack_elngth z = 0. Hence y = mode_cont [k'] sigma v.*)
+    induction .
+
+
+Lemma inversion_lemma:
+  forall x o l tj tc sigma v,
+  star cred
+    (mode_eval x [CDefault o l tj tc] sigma)
+    (mode_cont [] sigma v)
+  ->
+  exists v',
+  star cred
+    (mode_eval x [CDefault o l tj tc] sigma)
+    (mode_cont [CDefault o l tj tc] sigma v').
+Proof.
+
+
+Lemma thing1:
+  forall o x l tj tc sigma v,
+  star cred
+    (mode_cont ((CDefault o (x :: l) tj tc)::[]) sigma REmpty)
+    (mode_cont [] sigma v)
+  ->
+  star cred
+    (mode_cont ((CDefault o l tj tc)::[]) sigma REmpty)
+    (mode_eval (Default l tj tc) [] sigma).
+Proof.
+  intros.
+  inversion H; subst.
+  inversion H0; subst.
+  econstructor.
+  { eapply cred_defaultunpack. } 
+  do 2 econstructor.
+  { econstructor. }
+  - 
+  eapply star_step.
+
+
 
 
 (* semantics does no changes when permuting the differents exceptions *)
@@ -254,4 +408,11 @@ Theorem default_permut_stable ts1 ts2 tj tc sigma s1 s2:
   irred cred s2 ->
   s1 = s2.
 Proof.
-Abort.
+  induction 1.
+  * intros.
+    eapply finseq_unique; eauto using cred_deterministic.
+  * intros.
+    eapply IHPermutation; eauto.
+    - 
+
+Qed.
